first clean and doc WIP

src/module.v
@@ -1,138 +1,161 @@
-Require Import Bool.
 Require Import ZArith.
-Require dict hashtable.
+Require Import keys.
 Require Import Coq.Numbers.Cyclic.Int63.Uint63.
 Require Import List.
+Require radix table.
 
 Import ListNotations.
 
 Open Scope uint63_scope.
 
-Module Type Hash_type.
-  Parameter A: Set.
-  Parameter eq: A -> A -> bool.
-  Parameter eq_spec: forall x y : A, reflect (x = y) (eq x y).
-  Parameter hashp: A -> positive.
-  Parameter hashi: A -> int.
-End Hash_type.
+(** *** HashTablePositive: Hashtable with positive key (PATRICIA tree) *)
 
-Module Type HashTable (T : Hash_type).
-  Parameter t: Set -> Type.
-  Parameter create : forall B: Set, int -> t B.
-  Parameter add : forall {B:Set}, t B -> T.A -> B -> t B.
-  Parameter find : forall {B:Set}, t B -> T.A -> option B.
-  Parameter find_all: forall {B: Set}, t B -> T.A -> list B.
-  Parameter mem: forall {B: Set}, t B -> T.A -> bool.
-  Parameter remove: forall {B: Set}, t B -> T.A -> t B.
-  Parameter replace: forall {B: Set}, t B -> T.A -> B -> t B.
-
-  Parameter find_spec:
-    forall B (ht: t B) key,
-    find ht key = List.hd_error (find_all ht key).
-
-  Parameter hempty:
-    forall B k s, find (create B s) k = None.
-
-  Parameter add_same:
-    forall B k (h: t B) v,
-    find_all (add h k v) k = v :: (find_all h k).
-
-  Parameter add_diff:
-    forall B k k' (h: t B) v,
-    k' <> k -> find_all (add h k v) k' = find_all h k'.
-End HashTable.
-
-Module HashTableTree (T: Hash_type) <: HashTable T.
-  Definition t := @dict.t T.A.
+Module HashTablePositive (T: HashP).
+  Definition t := @radix.tree T.A.
   Definition create (B: Set) (_: int) : t B :=
-    dict.empty T.A B.
+    radix.empty T.A B.
 
-  Definition add {B: Set} (h: t B) (key: T.A) (v: B) :=
-    dict.add T.A B T.hashp key v h.
+  Definition add {B: Set} (h: t B) (k: T.A) (v: B) :=
+    radix.add T.A B T.hash h k v.
 
-  Definition find {B: Set} (h: t B) (key: T.A): option B :=
-    dict.find T.A T.eq B T.hashp key h.
+  Definition find {B: Set} (h: t B) (k: T.A): option B :=
+    radix.find T.A T.eq B T.hash h k.
 
-  Definition find_all {B: Set} (h: t B) (key: T.A) : list B :=
-    dict.find_all T.A T.eq B T.hashp key h.
+  Definition find_all {B: Set} (h: t B) (k: T.A) : list B :=
+    radix.find_all T.A T.eq B T.hash h k.
 
-  Definition remove {B: Set} (h: t B) (key: T.A) :=
-    dict.remove T.A T.eq B T.hashp key h.
+  Definition mem {B: Set} (h: t B) (k: T.A) : bool :=
+    radix.mem T.A T.eq B T.hash h k.
 
-  Definition replace {B: Set} (h: t B) (key: T.A) (v: B) :=
-    dict.replace T.A T.eq B T.hashp key v h.
+  Definition remove {B: Set} (h: t B) (k: T.A) :=
+    radix.remove T.A T.eq B T.hash h k.
 
-  Definition mem {B: Set} (h: t B) (key: T.A) : bool :=
-    match find h key with
-    | Some _ => true
-    | None   => false
-    end.
+  Definition replace {B: Set} (h: t B) (k: T.A) (v: B) :=
+    radix.replace T.A T.eq B T.hash h k v.
+
+  (** Facts *)
 
   Theorem find_spec:
-    forall B (ht: t B) key,
-    find ht key = List.hd_error (find_all ht key).
-  Admitted.
+    forall B (ht: t B) k,
+    find ht k = List.hd_error (find_all ht k).
+  Proof. intros *. apply radix.find_spec. Qed.
 
-  Theorem hempty:
+  Theorem find_empty:
     forall B k s, find (create B s) k = None.
-  Admitted.
+  Proof. intros *. apply radix.find_empty. Qed.
 
-  Theorem add_same:
-    forall B k (h: t B) v,
-    find_all (add h k v) k = v :: (find_all h k).
-  Admitted.
-
-  Theorem add_diff:
-    forall B k k' (h: t B) v,
-    k' <> k -> find_all (add h k v) k' = find_all h k'.
-  Admitted.
-End HashTableTree.
-
-Module HashTableBucket (T: Hash_type) <: HashTable T.
-  Definition t := @hashtable.t T.A.
-  Definition create (B: Set) (initial_size: int) : t B :=
-    @hashtable.create T.A B initial_size.
-
-  Definition add {B: Set} (h: t B) (key: T.A) (v: B) :=
-    hashtable.add T.hashi h key v.
-
-  Definition find {B: Set} (h: t B) (key: T.A): option B :=
-    hashtable.find T.eq T.hashi h key.
-
-  Definition find_all {B: Set} (h: t B) (key: T.A) :=
-    hashtable.find_all T.eq T.hashi h key.
-
-  Definition mem {B: Set} (h: t B) (key: T.A) :=
-    hashtable.mem  T.eq T.hashi h key.
-
-  Definition remove {B: Set} (h: t B) (key: T.A) :=
-    hashtable.remove T.eq T.hashi h key.
-
-  Definition replace {B: Set} (h: t B) (key: T.A) (v: B) :=
-    hashtable.replace T.eq T.hashi h key v.
-
-  Theorem find_spec:
-    forall B (ht: t B) key,
-    find ht key = List.hd_error (find_all ht key).
-  Proof. intros. apply hashtable.find_spec. Qed.
-
-  Theorem hempty:
-    forall B k s, find (create B s) k = None. 
-  Proof. intros. apply hashtable.hempty. Qed.
-
-  Theorem add_same:
-    forall B k (h: t B) v,
-    find_all (add h k v) k = v :: (find_all h k).
-  Proof. intros. apply hashtable.find_add_same, T.eq_spec. Qed.
-
-  Theorem add_diff:
-    forall B k k' (h: t B) v,
-    k' <> k -> find_all (add h k v) k' = find_all h k'.
+  Theorem mem_spec:
+    forall B (ht: t B) k v,
+    (find ht k = Some v -> mem ht k = true) /\
+    (find ht k = None   -> mem ht k = false).
   Proof.
-    intros B k k' h v H.
-    apply hashtable.find_add_diff.
-    apply T.eq_spec. apply H.
+    intros *.
+    split; unfold mem, find, radix.mem; now intros ->.
   Qed.
 
-End HashTableBucket.
+  Theorem add_same:
+    forall B (h: t B) k v,
+    find_all (add h k v) k = v :: (find_all h k).
+  Proof. intros *. apply radix.find_add_same. apply T.eq_spec. Qed.
+
+  Theorem add_other:
+    forall B (h: t B) k k' v,
+    k' <> k -> find_all (add h k v) k' = find_all h k'.
+  Proof. intros *. apply radix.find_add_other. apply T.eq_spec. Qed.
+
+  Theorem remove_same:
+    forall B (t: t B) k,
+    find_all (remove t k) k = List.tl (find_all t k).
+  Proof. intros *. apply radix.remove_same. Qed.
+
+  Theorem remove_other:
+    forall B (t: t B) k k',
+    k' <> k -> find_all (remove t k) k' = find_all t k'.
+  Proof. intros *. apply radix.remove_other. apply T.eq_spec. Qed.
+
+  Theorem replace_same:
+    forall B (ht: t B) k v,
+    find_all (replace ht k v) k = v :: (List.tl (find_all ht k)).
+  Proof. intros *. apply radix.replace_same. apply T.eq_spec. Qed.
+ 
+  Theorem replace_other:
+    forall B (ht: t B) k1 k2 v,
+    k1 <> k2 -> find_all (replace ht k1 v) k2 = find_all ht k2.
+  Proof. intros *. apply radix.replace_other. apply T.eq_spec. Qed.  
+
+End HashTablePositive.
+
+(** *** HashTable: Hashtable with PArray *)
+
+Module HashTable (T: HashI).
+  Definition t := @table.t T.A.
+  Definition create (B: Set) (initial_size: int) : t B :=
+    @table.create T.A B initial_size.
+
+  Definition add {B: Set} (h: t B) (key: T.A) (v: B) :=
+    table.add T.hash h key v.
+
+  Definition find {B: Set} (h: t B) (key: T.A): option B :=
+    table.find T.eq T.hash h key.
+
+  Definition find_all {B: Set} (h: t B) (key: T.A) :=
+    table.find_all T.eq T.hash h key.
+
+  Definition mem {B: Set} (h: t B) (key: T.A) :=
+    table.mem  T.eq T.hash h key.
+
+  Definition remove {B: Set} (h: t B) (key: T.A) :=
+    table.remove T.eq T.hash h key.
+
+  Definition replace {B: Set} (h: t B) (key: T.A) (v: B) :=
+    table.replace T.eq T.hash h key v.
+
+  (** Facts *)
+
+  Theorem find_spec:
+    forall B (ht: t B) key,
+    find ht key = List.hd_error (find_all ht key).
+  Proof. intros. apply table.find_spec. Qed.
+
+  Theorem find_empty:
+    forall B k s, find (create B s) k = None. 
+  Proof. intros. apply table.hempty. Qed.
+
+  Theorem mem_spec:
+    forall B (ht: t B) key v,
+    (find ht key = Some v -> mem ht key = true) /\
+    (find ht key = None   -> mem ht key = false).
+  Proof.
+    intros *.
+    split; unfold mem, find, table.mem; now intros ->.
+  Qed.
+
+  Theorem add_same:
+    forall B (h: t B) k v,
+    find_all (add h k v) k = v :: (find_all h k).
+  Proof. intros. apply table.find_add_same, T.eq_spec. Qed.
+
+  Theorem add_other:
+    forall B (h: t B) k k' v,
+    k' <> k -> find_all (add h k v) k' = find_all h k'.
+  Proof.
+    intros *. apply table.find_add_other. apply T.eq_spec.
+  Qed.
+
+  Theorem remove_same:
+    forall B (t: t B) k,
+    find_all (remove t k) k = List.tl (find_all t k).
+  Proof. intros *. apply table.remove_same. Qed.
+
+  Theorem remove_other:
+    forall B (t: t B) k k',
+    k' <> k -> find_all (remove t k) k' = find_all t k'.
+  Proof. intros *. apply table.remove_other. apply T.eq_spec. Qed.
+
+  Theorem replace_other:
+    forall B (ht: t B) k1 k2 v,
+    k1 <> k2 -> find_all (replace ht k1 v) k2 = find_all ht k2.
+  Proof. intros *. apply table.replace_other. apply T.eq_spec. Qed.  
+
+End HashTable.
 
