src/radix.v
@@ -1,54 +1,71 @@
 Require Import ZArith.
+Require Import Coq.ssr.ssrbool.
+Require Import int_utils.
+Require Import Coq.Lists.List.
+Import ListNotations.
 
 Open Scope positive_scope.
 
 Section Radix.
-  Context {A: Type}.
+  Variable A: Set.
+  Variable eq: A -> A -> bool.
+  Variable eq_spec: forall x y : A, reflect (x = y) (eq x y).
+  Variable B: Set.
+
+  Variable hash: A -> positive.
+
+  Inductive bucket : Set :=
+  | B_Empty : bucket
+  | B_Cons : positive -> A -> B -> bucket -> bucket.
 
   Inductive tree : Type :=
   | Empty: tree
-  | Node:  tree -> option A -> tree -> tree.
+  | Node:  tree -> bucket -> tree -> tree.
+
+  (** ** Tree functions *)
 
   Definition empty : tree := Empty.
   
-  Fixpoint get (p: positive) (t: tree) : option A :=
+  Fixpoint get (p: positive) (t: tree) : bucket :=
     match p, t with
-    | _,     Empty      => None
+    | _,     Empty      => B_Empty
     | xH,    Node _ e _ => e
     | xO p', Node l _ _ => get p' l
     | xI p', Node _ _ r => get p' r
     end.
 
-  Fixpoint set0 (p: positive) (e: A) : tree :=
+  Fixpoint set0 (p: positive) (e: bucket) : tree :=
     match p with
-    | xH    => Node Empty (Some e) Empty
-    | xO p' => Node (set0 p' e) None Empty
-    | xI p' => Node Empty None (set0 p' e)
+    | xH    => Node Empty e Empty
+    | xO p' => Node (set0 p' e) B_Empty Empty
+    | xI p' => Node Empty B_Empty (set0 p' e)
     end.
 
-  Fixpoint set (p: positive) (e: A) (t: tree) : tree :=
+  Fixpoint set (p: positive) (e: bucket) (t: tree) : tree :=
     match p, t with
     | _,     Empty      => set0 p e
-    | xH,    Node l _ r => Node l (Some e) r
+    | xH,    Node l _ r => Node l e r
     | xO p', Node l y r => Node (set p' e l) y r
     | xI p', Node l y r => Node l y (set p' e r)
     end.
 
+  (** ** Tree Facts *)
+
   Theorem gempty:
-    forall (i: positive), get i empty = None.
+    forall (i: positive), get i empty = B_Empty.
   Proof.
     intro i. case i; reflexivity.
   Qed.
 
   Theorem gss0:
-    forall (i: positive) (x: A), get i (set0 i x) = Some x.
+    forall (i: positive) (x: bucket), get i (set0 i x) = x.
   Proof.
     intros i x. induction i; simpl; auto.  
   Qed.
 
   Theorem gos0:
-    forall (i j: positive) (x: A), 
-    i <> j -> get i (set0 j x) = None.
+    forall (i j: positive) (x: bucket), 
+    i <> j -> get i (set0 j x) = B_Empty.
   Proof.
     induction i; intros j x H; simpl.
     - destruct j; simpl; [apply IHi; now intros <-| |]; apply gempty.
@@ -58,13 +75,13 @@ Section Radix.
 
 
   Theorem gss: 
-    forall (i: positive) (x: A) (t: tree), get i (set i x t) = Some x.
+    forall (i: positive) (x: bucket) (t: tree), get i (set i x t) = x.
   Proof.
     induction i; destruct t; simpl; auto; try apply IHi; now rewrite gss0.
   Qed.
 
   Theorem gso:
-    forall (i j: positive) (x: A) (t: tree),
+    forall (i j: positive) (x: bucket) (t: tree),
     i <> j -> get i (set j x t) = get i t.
   Proof.
     induction i; intros j x t H; destruct j, t;
@@ -75,6 +92,304 @@ Section Radix.
     - apply IHi. now intros <-.
   Qed.
 
+  (** ** hashtables functions *)
+
+  Fixpoint find_rec l h k: option B :=
+    match l with
+    | B_Empty => None
+    | B_Cons h' k' v tl =>
+        if if h =? h' then eq k k' else false
+        then Some v
+        else find_rec tl h k
+    end.
+
+  Definition find (t: tree) (k: A) : option B :=
+    let h := hash k in
+    find_rec (get h t) h k.
+
+  Fixpoint find_all_rec (l: bucket) (h: positive) (k: A) (acc: list B): list B :=
+    match l with
+    | B_Empty => List.rev' acc
+    | B_Cons h' k' v l' => 
+        if if h =? h' then eq k k' else false
+        then find_all_rec l' h k (v :: acc)
+        else find_all_rec l' h k acc
+    end.
+
+  Definition mem (h: tree) (key: A) : bool :=
+    match find h key with
+    | Some _ => true
+    | None   => false
+    end.
+
+  Definition find_all (d: tree) (k: A) : list B :=
+    let h_k := hash k in
+    find_all_rec (get h_k d) h_k k nil.
+
+  Definition add (d: tree) (k: A) (e: B) : tree :=
+    let h_k := hash k in
+    match get h_k d with
+    | B_Empty => set h_k (B_Cons h_k k e B_Empty) d
+    | b       => set h_k (B_Cons h_k k e b) d
+    end.
+
+  Fixpoint bucket_remove (b: bucket) (h: positive) (k: A) :=
+    match b with
+    | B_Empty => B_Empty
+    | B_Cons h' k' v b =>
+        if if h =? h' then eq k k' else false
+        then b
+        else B_Cons h' k' v (bucket_remove b h k)
+    end.
+
+  Definition remove (d: tree) (k: A) : tree :=
+    let h := hash k in
+    match get h d with
+    | B_Empty => d
+    | b       => set h (bucket_remove b h k) d
+    end.
+
+  Definition replace (d: tree) (k: A) (e: B) : tree :=
+    let h := hash k in
+    match get h d with
+    | B_Empty => set h (B_Cons h k e B_Empty) d
+    | b       => set h (B_Cons h k e (bucket_remove b h k)) d
+    end.
+
+  (** Eq *)
+
+  Lemma eq_true:
+    forall (k1 k2 : A), k1 = k2 -> eq k1 k2 = true.
+  Proof.
+    intros k1 k2 H.
+    now case eq_spec.
+  Qed.
+
+  Lemma eq_false:
+    forall (k1 k2 : A), k1 <> k2 -> eq k1 k2 = false.
+  Proof.
+    intros k1 k2 H.
+    now case eq_spec.
+  Qed.
+
+  Lemma eq_refl:
+    forall (k : A), k = k -> eq k k = true.
+  Proof.
+    intros k H.
+    now case eq_spec.
+  Qed.
+
+  (** find_all *)
+  Fixpoint find_all_rec' (l: bucket) (h: positive) (k: A) : list B :=
+    match l with
+    | B_Empty => nil
+    | B_Cons h' k' v l' =>
+        if if h =? h' then eq k k' else false
+        then v :: find_all_rec' l' h k
+        else find_all_rec' l' h k
+    end.
+
+  Lemma find_all_rec_correct:
+    forall (l: bucket) (h: positive) (key: A) acc,
+    find_all_rec l h key acc = rev acc ++ find_all_rec' l h key.
+  Proof.
+    intros l h k.
+    induction l.
+    + intros acc. simpl. apply rev_append_rev.
+    + intros acc. simpl. case (eq k a) eqn:H.
+      - case (h =? p).
+        * rewrite IHl. simpl. rewrite <- app_assoc. easy.
+        * simpl. apply IHl.
+      - case (h =? p).
+        * rewrite IHl. reflexivity.
+        * apply IHl.
+  Qed.
+
+  (** empty *)
+
+  Theorem find_empty:
+    forall (k: A), find empty k = None.
+  Proof.
+    intro i. unfold find.
+    assert (get (hash i) empty = B_Empty).
+    apply gempty. now rewrite H.
+  Qed.
+
+  (** add *)
+
+  Theorem find_add_same:
+    forall (d: tree) (k: A) (v: B),
+    find_all (add d k v) k = v :: find_all d k.
+  Proof.
+    intros d k x. unfold find_all, add.
+    rewrite 2!find_all_rec_correct. simpl.
+    case (get (hash k) d).
+    - rewrite gss. simpl.
+      case (eq_spec k k). intros Hk.
+      assert (H: hash k =? hash k = true) by now rewrite Pos.eqb_eq.
+      now rewrite H.
+      intros Hk. contradiction.
+    - intros *. rewrite gss. simpl.
+      case (eq_spec k k); intros Hk. 2:contradiction.
+      assert (H: hash k =? hash k = true) by now rewrite Pos.eqb_eq.
+      now rewrite H.
+  Qed.
+
+  Theorem find_add_other:
+    forall (d: tree) (k k': A) (v: B),
+    k' <> k -> find_all (add d k v) k' = find_all d k'.
+  Proof.
+    intros d k k' v. intros Hk. unfold find_all, add.
+    rewrite 2!find_all_rec_correct. simpl.
+    case (hash k =? hash k') eqn:Hh.
+    - apply Peqb_true_eq in Hh. rewrite Hh. case (get (hash k') d).
+      * rewrite gss. simpl. rewrite Pos.eqb_refl.
+        now rewrite (eq_false k' k Hk).
+      * intros *. rewrite gss.
+        simpl. rewrite Pos.eqb_refl. now rewrite (eq_false k' k Hk).
+    - rewrite Pos.eqb_neq in Hh. case (get (hash k) d).
+      * rewrite gso. easy.
+        intros H; apply Hh; now rewrite H.
+      * intros *. rewrite gso. easy.
+        intros H; apply Hh; now rewrite H.
+  Qed.
+
+  (** find *)
+
+  Theorem find_spec:
+    forall t key,
+    find t key = List.hd_error (find_all t key).
+  Proof.
+    intros t key.
+    unfold find_all, find.
+    induction (get (hash key) t). easy.
+    simpl. case (if hash key =? p then eq key a else false).
+    + now rewrite find_all_rec_correct.
+    + apply IHb.
+  Qed.
+
+  (** remove  *)
+
+  Lemma bucket_remove_same:
+    forall (b: bucket) (k: A),
+    let h := hash k in
+    find_all_rec (bucket_remove b h k) h k []  =
+    List.tl (find_all_rec b h k []).
+  Proof.
+    induction b; intros k h. easy. simpl.
+    case (if h =? p then eq k a else false) eqn:Hc.
+    + destruct (h =? p); try easy.
+      rewrite 2!find_all_rec_correct. easy.
+    + simpl. rewrite Hc. apply IHb.
+  Qed.
+
+  Lemma bucket_remove_other:
+    forall (b: bucket) (k k': A),
+    let h := hash k in
+    let h' := hash k' in
+    k' <> k ->
+    find_all_rec (bucket_remove b h k) h' k' []  =
+    find_all_rec b h' k' [].
+  Proof.
+    induction b; intros k k' h h' Hk. easy. simpl.
+    case (if h =? p then eq k a else false) eqn:Hc; simpl.
+    + assert ((if h' =? p then eq k' a else false) = false).
+      { case (h' =? p). 2:easy. apply eq_false.
+        assert (Hkb: eq k a = true). case (h =? p) in Hc; easy.
+        case (eq_spec k a) in Hkb; try discriminate.
+        rewrite <- e. apply Hk. }
+      rewrite H. reflexivity.
+    + case (if h' =? p then eq k' a else false).
+      - rewrite 2!find_all_rec_correct. f_equal.
+        rewrite <- app_nil_l at 1. rewrite <- app_nil_l.
+        assert (H:@rev (list B) [] = []). reflexivity.
+        change [] with (@rev B []).
+        rewrite <- 2!find_all_rec_correct. apply IHb. exact Hk.
+      - apply IHb. exact Hk.
+  Qed.
+
+  Theorem remove_same:
+    forall (t: tree) (k: A),
+    find_all (remove t k) k =
+    List.tl (find_all t k).
+  Proof.
+    intros t k. unfold remove, find_all.
+    rewrite 2!find_all_rec_correct. simpl.
+    case (get (hash k) t) eqn:H. now rewrite H.
+    generalize (bucket_remove_same (get (hash k) t) k). simpl.
+    case (if hash k =? p then eq k a else false) eqn:Heq.
+    + simpl. now rewrite gss.
+    + simpl. rewrite 2!find_all_rec_correct. rewrite H. simpl.
+      rewrite gss. simpl. rewrite Heq. simpl. now rewrite Heq.
+  Qed.
+
+  Theorem remove_other:
+    forall (t: tree) (k: A) (k': A),
+    k' <> k ->
+    find_all (remove t k) k' = find_all t k'.
+  Proof.
+    intros *. unfold remove, find_all. intros Hk.
+    case (get (hash k) t) eqn:H. easy.
+    case (hash k =? hash k') eqn:Hh.
+    + apply Peqb_true_eq in Hh. rewrite Hh at 1. rewrite gss.
+      rewrite bucket_remove_other. 2:easy. rewrite <- Hh. now rewrite H.
+    + rewrite gso. easy. apply not_eq_sym. now apply Pos.eqb_neq.
+  Qed.
+
+
+  (** replace *)
+
+  Theorem replace_same:
+    forall h key v,
+    find_all (replace h key v) key = v :: (List.tl (find_all h key)).
+  Proof.
+    intros h key v. unfold find_all, replace.
+    case (get (hash key) h).
+    + rewrite gss. simpl. now rewrite Pos.eqb_refl, eq_refl.
+    + intros *. rewrite gss. simpl. rewrite Pos.eqb_refl, eq_refl. 2: easy.
+      f_equal. case (if hash key =? p then eq key a else false) eqn:H.
+      * rewrite 2!find_all_rec_correct. reflexivity.
+      * simpl. rewrite H. rewrite <- bucket_remove_same, 2!find_all_rec_correct.
+        reflexivity.
+  Qed.
+
+  Theorem replace_other:
+    forall h k1 k2 v,
+    k1 <> k2 ->
+    find_all (replace h k1 v) k2 = find_all h k2.
+  Proof.
+    intros h k1 k2 v Hk. unfold find_all, replace.
+    case (hash k1 =? hash k2) eqn:Hh.
+    + case (get (hash k1) h) eqn:Hg; apply Peqb_true_eq in Hh.
+      * rewrite 2!find_all_rec_correct. simpl.
+        rewrite <- Hh, Hg. rewrite gss. simpl.
+        rewrite Pos.eqb_refl, eq_false. easy.
+        now apply not_eq_sym.
+      * rewrite Hh. rewrite gss.
+        simpl. rewrite Pos.eqb_refl, eq_false.
+        2:intros H; apply Hk; now rewrite H.
+        rewrite <- Hh, Hg. simpl.
+        case (hash k1 =? p) eqn:Heq.
+        - case (eq k1 a) eqn:Hk1.
+          **rewrite eq_false. easy.
+            case (eq_spec k1 a) in Hk1; try discriminate.
+            rewrite <- e. now apply not_eq_sym.
+          **simpl. rewrite Heq.
+            generalize (bucket_remove_other b0 k1 k2). simpl.
+            rewrite 6!find_all_rec_correct. simpl. intros H.
+            case (eq k2 a). f_equal.
+            all: rewrite Hh at 2; rewrite H, Hh. 1,3: easy.
+            all: now apply not_eq_sym.
+        - simpl. rewrite Hh at 5. rewrite bucket_remove_other.
+          now rewrite Heq, Hh. now apply not_eq_sym.
+    + case (get (hash k1) h).
+      * rewrite gso. easy.
+        apply Pos.eqb_neq in Hh.
+        apply (not_eq_sym Hh).
+      * intros *. rewrite gso. easy.
+        apply Pos.eqb_neq in Hh.
+        apply (not_eq_sym Hh).
+  Qed.
 End Radix.
 
 Arguments tree A : clear implicits.
